refactor: fix imports

src/Equivalence/BigStepToFrameStack/WellFormedMap.v
@@ -1,29 +1,67 @@
 From CoreErlang.BigStep Require Import BigStep.
 From CoreErlang.FrameStack Require Import SubstSemantics.
-
 Require Import stdpp.list.
 
 Import BigStep.
 
-Definition well_formed_map (v : Value) : Prop :=
-    match v with
-    | VMap vl => vl = 
-      let (f , l) := (make_value_map (fst (split vl)) (snd (split vl)))
-      in zip f l
-    | _ => True
-    end.
+(**
+* well_formed_map_bs
+* well_formed_map_fs
+*)
 
-   Fixpoint well_formed_map_framestack (v : Val) : Prop :=
-   match v with
-   | Syntax.VNil => True
-   | Syntax.VLit l => True
-   | VPid p => True
-   | Syntax.VCons hd tl => well_formed_map_framestack hd /\ well_formed_map_framestack tl
-   | Syntax.VTuple l => foldr (fun v acc => well_formed_map_framestack v /\ acc) True l
-   | Syntax.VMap l => l = make_val_map l 
-      /\ foldr (fun v acc => PBoth well_formed_map_framestack v /\ acc) True l
-   (* /\ Forall (PBoth well_formed_map_framestack) l *)
-   | VVar n => True
-   | VFunId n => True
-   | Syntax.VClos ext id params e => True
-  end.
+(**
+NOTES:  Later change lists to maps in Syntax
+*)
+
+
+
+Definition well_formed_map_bs
+  (v : Value)
+  : Prop
+  :=
+match v with
+| VMap vl =>
+    vl
+    =
+    let (f , l) :=
+      (make_value_map
+        (fst (split vl)) 
+        (snd (split vl)))
+    in zip f l
+
+| _ => True
+end.
+
+
+
+
+
+
+Fixpoint well_formed_map_fs
+  (v : Val)
+  : Prop
+  :=
+match v with
+| Syntax.VCons hd tl =>
+    well_formed_map_fs hd
+    /\
+    well_formed_map_fs tl
+
+| Syntax.VTuple l =>
+    foldr
+      (fun v acc =>
+        well_formed_map_fs v /\ acc)
+      True 
+      l
+
+| Syntax.VMap l =>
+    l = make_val_map l
+    /\
+    foldr
+      (fun v acc =>
+        PBoth well_formed_map_fs v /\ acc)
+      True
+      l
+
+| _ => True
+end.
