src/Equivalence/BigStepToFrameStack/EnvironmentLemmas.v
@@ -1,19 +1,26 @@
-From CoreErlang.BigStep Require Import Environment.
+From CoreErlang.BigStep Require Export Environment.
 
-
-
-(* NOTE: maybe place this in BigStep/Environment *)
+From CoreErlang Require Import Basics.
+Require Import stdpp.list.
 
 (**
-
 * Help
-  - env_rem
+  - Remove
+    + env_rem
+  - Get
+    + get_value_cons
 * Main
-  - env_rem_vars
-  - env_rem_fids
-  - env_rem_fids_vars
-  - env_rem_ext
+  - Remove
+    + env_rem_vars
+    + env_rem_fids
+    + env_rem_fids_vars
+    + env_rem_ext
+  - Get
+    + can_get_value_than_in
+*)
 
+(**
+NOTES:  Maybe place this in BigStep/Environment
 *)
 
 
@@ -22,18 +29,61 @@ Section Help.
 
 
 
-  Definition env_rem
-    (keys : list (Var + FunctionIdentifier))
-    (env : Environment)
-    : Environment
-    :=
-  fold_left
-    (fun env' key =>
-      filter (fun '(k, v) =>
-        negb (var_funid_eqb k key))
-        env')
-    keys
-    env.
+  Section Remove.
+
+    Definition env_rem
+      (keys : list (Var + FunctionIdentifier))
+      (env : Environment)
+      : Environment
+      :=
+    fold_left
+      (fun env' key =>
+        filter (fun '(k, v) =>
+          negb (var_funid_eqb k key))
+          env')
+      keys
+      env.
+
+  End Remove.
+
+
+
+  Section Get.
+
+    Theorem get_value_cons :
+      forall env key k var v,
+          get_value ((k, v) :: env) key = Some [var]
+      ->  get_value [(k, v)] key = Some [var] 
+      \/
+          get_value env key = Some [var].
+    Proof.
+      intros env key k var v Hcons.
+      unfold get_value in Hcons.
+      remember
+        (var_funid_eqb key k)
+        as _key_eqb.
+      symmetry in Heq_key_eqb.
+      destruct _key_eqb.
+      * left.
+        clear env.
+        inv Hcons.
+        unfold var_funid_eqb in Heq_key_eqb.
+        destruct key.
+        - destruct k.
+          + cbn.
+            rewrite Heq_key_eqb.
+            reflexivity.
+          + congruence.
+        - destruct k.
+          + congruence.
+          + cbn.
+            rewrite Heq_key_eqb.
+            reflexivity.
+      * right.
+        exact Hcons.
+    Qed.
+
+  End Get.
 
 
 
@@ -48,40 +98,85 @@ Section Main.
 
 
 
-  Definition env_rem_vars
-    (vars : list Var)
-    (env : Environment)
-    : Environment
-    :=
-  env_rem (map inl vars) env.
+  Section Remove.
+
+    Definition env_rem_vars
+      (vars : list Var)
+      (env : Environment)
+      : Environment
+      :=
+    env_rem (map inl vars) env.
 
 
 
-  Definition env_rem_fids
-    (fids : list (FunctionIdentifier * FunctionExpression))
-    (env : Environment)
-    : Environment
-    :=
-  env_rem (map inr (map fst fids)) env.
+    Definition env_rem_fids
+      (fids : list (FunctionIdentifier * FunctionExpression))
+      (env : Environment)
+      : Environment
+      :=
+    env_rem (map inr (map fst fids)) env.
 
 
 
-  Definition env_rem_fids_vars
-    (fids : list (FunctionIdentifier * FunctionExpression))
-    (vars : list Var)
-    (env : Environment)
-    : Environment
-    :=
-  env_rem_fids fids (env_rem_vars vars env).
+    Definition env_rem_fids_vars
+      (fids : list (FunctionIdentifier * FunctionExpression))
+      (vars : list Var)
+      (env : Environment)
+      : Environment
+      :=
+    env_rem_fids fids (env_rem_vars vars env).
 
 
 
-  Definition env_rem_ext
-    (ext : list (nat * FunctionIdentifier * FunctionExpression))
-    (env : Environment)
-    : Environment
-    :=
-  env_rem (map inr (map snd (map fst ext))) env.
+    Definition env_rem_ext
+      (ext : list (nat * FunctionIdentifier * FunctionExpression))
+      (env : Environment)
+      : Environment
+      :=
+    env_rem (map inr (map snd (map fst ext))) env.
+
+  End Remove.
+
+
+
+  Section Get.
+
+    Theorem can_get_value_than_in :
+      forall env key var,
+          get_value env key = Some [var]
+      ->  In (key , var) env.
+    Proof.
+      intros env.
+      induction env; intros key var Hget_value.
+      * inv Hget_value.
+      * destruct a as [k v].
+        apply get_value_cons in Hget_value.
+        destruct Hget_value.
+        - clear IHenv.
+          rename H into Hget_value.
+          unfold get_value in Hget_value.
+          remember
+            (var_funid_eqb key k)
+            as _key_eqb.
+          symmetry in Heq_key_eqb.
+          destruct _key_eqb.
+          + inv Hget_value.
+            apply var_funid_eqb_eq in Heq_key_eqb.
+            rewrite <- Heq_key_eqb.
+            clear Heq_key_eqb k.
+            constructor.
+            clear env.
+            reflexivity.
+          + clear Heq_key_eqb.
+            congruence.
+        - rename H into Hget_value.
+          specialize (IHenv key var Hget_value).
+          pose proof in_cons (k, v) (key, var) env IHenv.
+          clear IHenv Hget_value.
+          assumption.
+    Qed.
+
+  End Get.
 
 
 
