src/Equivalence/BigStepToFrameStack/FrameStackLemmas.v
@@ -1,69 +1,102 @@
-From CoreErlang.FrameStack Require Import SubstSemanticsLemmas.
+From CoreErlang.FrameStack Require Export SubstSemanticsLemmas.
 
 Require Import stdpp.list.
 
+(**
+* framestack_ident
+* framestack_ident_rev [Admitted]
+*)
+
+(**
+Note: Maybe place this into CoreErlang.FrameStack/SubstSemanticsLemmas
+*)
 
 
-  Theorem framestack_ident :
-    forall ident el vl vl' r x eff Fs,
+
+Theorem framestack_ident :
+  forall ident el vl vl' r x eff Fs,
       create_result ident (vl ++ x :: vl') [] = Some (r , eff)
-      -> list_biforall (fun e v => ⟨ [] , RExp e ⟩ -->* RValSeq [v]) el vl'
-      -> exists k, ⟨ FParams ident vl el :: Fs, RValSeq [x] ⟩ -[ k ]-> ⟨ Fs, r ⟩.
-  Proof.
-    intros.
-    generalize dependent r. generalize dependent vl'. revert vl. revert x.
-    induction el; intros.
+  ->  list_biforall
+        (fun e v => ⟨ [] , RExp e ⟩ -->* RValSeq [v]) 
+        el 
+        vl'
+  ->  exists k, 
+        ⟨ FParams ident vl el :: Fs, RValSeq [x] ⟩ -[ k ]-> ⟨ Fs, r ⟩.
+Proof.
+  intros ident el vl vl' r x eff Fs Hcreate Hbiforall.
+  generalize dependent r.
+  generalize dependent vl'.
+  revert vl.
+  revert x.
+  induction el; intros.
+  * inv Hbiforall.
+    exists 1.
+    econstructor.
+    econstructor.
+    by symmetry.
+    constructor.
+  * inv Hbiforall.
+    rename H3 into Hbiforall.
+    destruct H1 as [khd [Hhd Dhd]].
+    replace
+      (vl ++ x :: hd' :: tl') with
+      ((vl ++ [x]) ++ hd' :: tl') 
+      in Hcreate.
+    2:
     {
-      inv H0.
-      exists 1. econstructor. econstructor. by symmetry.
-      constructor.
+      rewrite <- app_assoc.
+      by rewrite <- app_cons_swap.
     }
-    {
-      inv H0.
-      destruct H3 as [khd [Hhd Dhd]].
-      replace (vl ++ x :: hd' :: tl') with ((vl ++ [x]) ++ hd' :: tl') in H.
-      2: {
-        rewrite <- app_assoc.
-        by rewrite <- app_cons_swap.
-      }
-      specialize (IHel _ _ _ H5 _ H). destruct IHel as [kIH DIH].
-      eexists. econstructor. constructor.
-      eapply transitive_eval.
-      eapply frame_indep_core in Dhd. exact Dhd.
-      simpl. exact DIH.
-    }
-  Qed.
+    specialize (IHel _ _ _ Hbiforall _ Hcreate).
+    destruct IHel as [kIH DIH].
+    eexists. 
+    econstructor. 
+    constructor.
+    eapply transitive_eval.
+    eapply frame_indep_core in Dhd. 
+    exact Dhd.
+    simpl.
+    exact DIH.
+Qed.
 
-  Theorem framestack_ident_rev :
-    forall el ident vl e k r,
-     ⟨ [FParams ident vl el], RExp e ⟩ -[ k ]-> ⟨ [], RValSeq r ⟩
-     -> exists v vl' eff, 
-          create_result ident (vl ++ v :: vl') [] = Some (RValSeq r, eff) /\ 
-          list_biforall (λ (e0 : Exp) (v : Val), ⟨ [], RExp e0 ⟩ -->* RValSeq [v]) (e :: el) (v :: vl').
-  Proof.
-    induction el; intros.
-    * Search step_rt.
-      pose proof term_eval.
-      pose proof terminates_in_k_eq_terminates_in_k_sem.
-      unfold terminates_in_k_sem in H1.
-      assert (is_result r).
-      {
-        constructor.
-        admit. (*scope *)
-      }
-      pose proof conj H2 H.
-      apply ex_intro with (x := RValSeq r) in H3.
-      apply H1 in H3.
-      apply H0 in H3. 2:
-      {
-        admit. (* scope *)
-      }
-      destruct H3 as [v [k0 [Hres [Hv Hk]]]].
-      inv Hres.
-      {
-        pose proof transitive_eval_rev. (* H Hv *) (* inv H*)
-        admit.
-      }
+
+
+
+
+
+Theorem framestack_ident_rev :
+  forall el ident vl e k r,
+      ⟨ [FParams ident vl el], RExp e ⟩ -[ k ]-> ⟨ [], RValSeq r ⟩
+  ->  exists v vl' eff,
+          create_result ident (vl ++ v :: vl') [] = Some (RValSeq r, eff)
+      /\  list_biforall 
+            (λ (e0 : Exp) (v : Val), ⟨ [], RExp e0 ⟩ -->* RValSeq [v])
+            (e :: el)
+            (v :: vl').
+Proof.
+  induction el; intros.
+  * Search step_rt.
+    pose proof term_eval.
+    pose proof terminates_in_k_eq_terminates_in_k_sem.
+    unfold terminates_in_k_sem in H1.
+    assert (is_result r).
+    {
+      constructor.
+      admit. (*scope *)
+    }
+    pose proof conj H2 H.
+    apply ex_intro with (x := RValSeq r) in H3.
+    apply H1 in H3.
+    apply H0 in H3. 2:
+    {
+      admit. (* scope *)
+    }
+    destruct H3 as [v [k0 [Hres [Hv Hk]]]].
+    inv Hres.
+    {
+      pose proof transitive_eval_rev. (* H Hv *) (* inv H*)
       admit.
-    * admit.
-  Admitted.
+    }
+    admit.
+  * admit.
+Admitted.
