src/Equivalence/BigStepToFrameStack/ScopingLemmas.v
@@ -1,46 +1,66 @@
-From CoreErlang.FrameStack Require Import SubstSemanticsLemmas.
+From CoreErlang.FrameStack Require Export SubstSemantics.
 
 Require Import stdpp.list.
 
+Import SubstSemantics.
+
+(**
+* scope_vl_succ
+* scope_vl_succ_id
+*)
+
+(**
+NOTES:  Maybe place this in CoreFrameStack/Scoping! or into FrameStack
+*)
 
 
-  Theorem scope_vl_succ :
-    forall A i vl (f : A -> Val),
-      (∀ i : nat, i < base.length vl →  VALCLOSED (nth i (map f vl) Syntax.VNil))
-      -> (S i < S (base.length vl) →  VALCLOSED (nth i (map f vl) Syntax.VNil)).
-  Proof.
-    intros A i vl f Hvl.
-    specialize (Hvl i).
-    intros Hsucc_lt.
-    pose proof Nat.succ_lt_mono as Hmono_succ_lt.
-    specialize (Hmono_succ_lt i (base.length vl)).
-    destruct Hmono_succ_lt as [Hto_succ_lt Hfrom_succ_lt].
-    clear Hto_succ_lt.
-    apply Hfrom_succ_lt in Hsucc_lt as Hlt.
-    clear Hfrom_succ_lt Hsucc_lt.
-    apply Hvl in Hlt.
-    clear Hvl.
-    rename Hlt into Hvl.
-    exact Hvl.
-  Qed.
 
-  Theorem scope_vl_succ_id :
-    forall i vl,
-      (∀ i : nat, i < base.length vl →  VALCLOSED (nth i vl Syntax.VNil))
-      -> (S i < S (base.length vl) →  VALCLOSED (nth i vl Syntax.VNil)).
-  Proof.
-    intros i vl Hvl.
-    assert (map id vl = vl).
-    {
-      apply Basics.map_id.
-    }
-    remember
-      (base.length vl)
-      as _n.
-    rewrite <- H.
-    rewrite <- H in Hvl.
-    rewrite Heq_n in *.
-    clear Heq_n _n H.
-    pose proof scope_vl_succ Val i vl id Hvl.
-    assumption.
-  Qed.
+Theorem scope_vl_succ :
+  forall A i vl (f : A -> Val),
+     (∀ i : nat, i < length vl → VALCLOSED (nth i (map f vl) VNil))
+  ->  (S i < S (length vl) → VALCLOSED (nth i (map f vl) VNil)).
+Proof.
+  intros A i vl f Hvl.
+  specialize (Hvl i).
+  intros Hsucc_lt.
+  pose proof Nat.succ_lt_mono 
+    as Hmono_succ_lt.
+  specialize (Hmono_succ_lt i (base.length vl)).
+  destruct Hmono_succ_lt
+    as [Hto_succ_lt Hfrom_succ_lt].
+  clear Hto_succ_lt.
+  apply Hfrom_succ_lt
+    in Hsucc_lt 
+    as Hlt.
+  clear Hfrom_succ_lt Hsucc_lt.
+  apply Hvl in Hlt.
+  clear Hvl.
+  rename Hlt into Hvl.
+  exact Hvl.
+Qed.
+
+
+
+
+
+
+Theorem scope_vl_succ_id :
+  forall i vl,
+    (∀ i : nat, i < length vl → VALCLOSED (nth i vl VNil))
+    -> (S i < S (length vl) → VALCLOSED (nth i vl VNil)).
+Proof.
+  intros i vl Hvl.
+  assert (map id vl = vl).
+  {
+    apply Basics.map_id.
+  }
+  remember
+    (base.length vl)
+    as _n.
+  rewrite <- H.
+  rewrite <- H in Hvl.
+  rewrite Heq_n in *.
+  clear Heq_n _n H.
+  pose proof scope_vl_succ Val i vl id Hvl.
+  assumption.
+Qed.
