src/Equivalence/BigStepToFrameStack/Simple/Tactics.v
@@ -1,50 +1,84 @@
-From CoreErlang.Equivalence.BigStepToFrameStack Require Import Measure.
-From CoreErlang.Equivalence.BigStepToFrameStack.Simple Require Import Substitute.
+From CoreErlang.Equivalence.BigStepToFrameStack.Simple Require Export MeasureLemmas.
 
-Ltac do_step
-  :=
-econstructor;
-[constructor;auto| simpl].
+(**
+* Basics
+  - do_step [Exists]
+  - clear_refl
+* Remember
+  - rmb_sbt_mval
+  - rmb_sbt_mval_tmp
+  - rmb_sbt_mval_spl
+  - rmb_sbt_mval_spl_step
+*)
 
-Ltac clear_refl
-  :=
-repeat match goal with
-| H : ?x = ?x |- _ => clear H
-end.
+(**
+Note: Move Basics to CoreErlangBasics
+*)
 
-Ltac rmb_sbt_mval
-  v     (* : Value *)
-  name  (* remember as *)
-  Hname (* remember eqn *)
-  :=
-remember
-  (subst_env (measure_val v))
-  as name
-  eqn:Hname.
 
-Ltac rmb_sbt_mval_tmp
-  v (* : Value *)
-  :=
-remember
-  (subst_env (measure_val v))
-  as _tmp
-  eqn:Heq_tmp.
 
-Ltac rmb_sbt_mval_spl
-  v (* : Value *)
-  :=
-rmb_sbt_mval_tmp v;
-simpl;
-inversion Heq_tmp;
-subst;
-clear_refl.
+(* Basics *)
 
-Ltac rmb_sbt_mval_spl_step
-  v (* : Value *)
-  :=
-rmb_sbt_mval_tmp v;
-simpl;
-do_step;
-inversion Heq_tmp;
-subst;
-clear_refl.
+
+
+  Ltac do_step
+    :=
+  econstructor;
+  [constructor;auto| simpl].
+
+
+
+  Ltac clear_refl
+    :=
+  repeat match goal with
+  | H : ?x = ?x |- _ => clear H
+  end.
+
+
+
+(* Remember *)
+
+
+
+  Ltac rmb_sbt_mval
+    v     (* : Value *)
+    name  (* remember as *)
+    Hname (* remember eqn *)
+    :=
+  remember
+    (subst_env (measure_val v))
+    as name
+    eqn:Hname.
+
+
+
+  Ltac rmb_sbt_mval_tmp
+    v (* : Value *)
+    :=
+  remember
+    (subst_env (measure_val v))
+    as _tmp
+    eqn:Heq_tmp.
+
+
+
+  Ltac rmb_sbt_mval_spl
+    v (* : Value *)
+    :=
+  rmb_sbt_mval_tmp v;
+  simpl;
+  inversion Heq_tmp;
+  subst;
+  clear_refl.
+
+
+
+  Ltac rmb_sbt_mval_spl_step
+    v (* : Value *)
+    :=
+  rmb_sbt_mval_tmp v;
+  simpl;
+  do_step;
+  inversion Heq_tmp;
+  subst;
+  clear_refl.
