src/Equivalence/BigStepToFrameStack/WellFormedMapLemmas.v
@@ -1,0 +1,180 @@
+From CoreErlang.Equivalence.BigStepToFrameStack Require Export WellFormedMap.
+
+From CoreErlang.FrameStack Require Import SubstSemantics.
+Require Import stdpp.list.
+
+Import SubstSemantics.
+
+(**
+* Help
+  - make_val_map_length [Admitted]
+  - make_val_map_cons
+* Main
+  - well_formed_map_fs_tuple
+  - well_formed_map_fs_map
+*)
+
+(**
+NOTES:  Later change lists to maps in Syntax
+*)
+
+
+
+Section Help.
+
+
+
+  Theorem make_val_map_length :
+    forall ms,
+      length (make_val_map ms) <= length ms.
+  Proof.
+    induction ms as [| (k, v) ms' IHms'].
+    - (* Base case: ms = [] *)
+      simpl.
+      apply le_n.
+    - (* Inductive case: ms = (k, v) :: ms' *)
+      simpl.
+      destruct
+        (make_val_map ms')
+        as [| (k', v') ms'']
+        eqn:Hmap.
+      + (* Case: make_val_map ms' = [] *)
+        simpl in IHms'.
+        by apply le_n_S.
+      + (* Case: make_val_map ms' = (k', v') :: ms'' *)
+        simpl.
+        destruct (k <ᵥ k') eqn:Hlt.
+        * (* Case: k <ᵥ k' *)
+          clear Hmap Hlt.
+          simpl.
+          apply le_n_S.
+          apply IHms'.
+        * destruct (k =ᵥ k') eqn:Heq.
+          -- (* Case: k =ᵥ k' *)
+             clear Hmap Hlt Heq.
+             simpl.
+             apply le_S.
+             apply IHms'.
+          -- (* Case: k >ᵥ k' *)
+             simpl.
+             admit.
+  Admitted.
+
+
+
+  Theorem make_val_map_cons :
+    forall v1 v2 vl,
+      (v1, v2) :: vl = make_val_map ((v1, v2) :: vl)
+      -> vl = make_val_map vl.
+  Proof.
+    intros v1 v2 vl H.
+    inv H.
+    rename H1 into H.
+    unfold Maps.map_insert in H.
+    destruct
+      (make_val_map vl)
+      as [| (k', v') vl']
+      eqn:Hmap.
+    - (* Case: make_val_map vl = [] *)
+      clear Hmap.
+      by inv H.
+    - (* Case: make_val_map vl = (k', v') :: ms *)
+      destruct (v1 <ᵥ k') eqn:Hlt.
+      + (* Case: v1 <ᵥ k' *)
+        clear Hlt.
+        by inv H.
+      + destruct (v1 =ᵥ k') eqn:Heq.
+        * (* Case: v1 =ᵥ k' *)
+          clear Hlt Heq.
+          inv H.
+          pose proof make_val_map_length vl' as Hlength.
+          rewrite Hmap in Hlength.
+          simpl in Hlength.
+          lia.
+        * (* Case: v1 >ᵥ k' *)
+          clear Hmap Hlt.
+          inv H.
+          rewrite Val_eqb_refl in Heq.
+          congruence.
+  Qed.
+
+
+
+End Help.
+
+
+
+
+
+
+Section Main.
+
+
+
+  Theorem well_formed_map_fs_tuple :
+    forall v vl,
+        Forall well_formed_map_fs [VTuple (v :: vl)]
+    ->  Forall well_formed_map_fs [v]
+    /\  Forall well_formed_map_fs [VTuple vl].
+  Proof.
+    intros v vl Hvvl.
+    inv Hvvl.
+    clear H2.
+    destruct H1.
+    rename H into Hv.
+    rename H0 into Hvl.
+    split.
+    - apply Forall_cons.
+      + exact Hv.
+      + apply Forall_nil.
+    - apply Forall_cons.
+      + unfold well_formed_map_fs.
+        exact Hvl.
+      + apply Forall_nil.
+  Qed.
+
+
+
+  Theorem well_formed_map_fs_map :
+    forall v1 v2 vl,
+        Forall well_formed_map_fs [VMap ((v1, v2) :: vl)]
+    ->  Forall well_formed_map_fs [v1]
+    /\  Forall well_formed_map_fs [v2]
+    /\  Forall well_formed_map_fs [VMap vl].
+  Proof.
+    intros v1 v2 vl Hv1v2vl.
+    inv Hv1v2vl.
+    clear H2.
+    destruct H1.
+    inv H0.
+    inv H1.
+    rename H0 into Hv1.
+    rename H3 into Hv2.
+    rename H2 into Hvl.
+    rename H into Hmap.
+    cbn in Hv1.
+    cbn in Hv2.
+    split.
+    - apply Forall_cons.
+      + exact Hv1.
+      + apply Forall_nil.
+    - clear Hv1.
+      split.
+      + apply Forall_cons. 
+        * exact Hv2.
+        * apply Forall_nil.
+      + clear Hv2.
+        apply Forall_cons.
+        * unfold well_formed_map_fs.
+          split. 2:
+          {
+            exact Hvl.
+          }
+          clear Hvl.
+          by pose proof make_val_map_cons v1 v2 vl Hmap.
+       * apply Forall_nil.
+  Qed.
+
+
+
+End Main.
